proof/theories/Generated/Router_Gen.v
@@ -1,21 +1,62 @@
 (* AUTO-GENERATED from ../../rulesets/router.nft by nft2coq (extracted/nft_emit.ml). DO NOT EDIT.
-   This is the parser's output as Coq terms: the chains and the set/map
-   declarations their lookups read.  Properties proved about these terms
-   are properties of the parsed ruleset (and, via compile_table_correct, of
-   the installed bytecode). *)
+   This is the parser's SURFACE output as a Coq [sruleset]; the tables,
+   chains, hooks and set/map declarations the proofs reason about are the
+   VERIFIED lowering [Lower.lower_ruleset] applied to it (no hand-written
+   bytes here).  A refused construct fails [router_lowers_ok] (fail-loud). *)
 
 From Stdlib Require Import List String ZArith.
 From Nft Require Import Bytes Verdict Packet Bytecode Syntax Semantics Nftval Elab.
+From Nft Require Import Surface.Ast Surface.Lower Gen_Support.
 Import ListNotations.
 Open Scope string_scope.
 
-Definition decls : set_decls :=
-  {| sd_sets := [];
-   sd_vmaps := [("__map0", [([6; 0; 22], [6; 0; 22], Accept); ([17; 0; 53], [17; 0; 53], Accept); ([6; 0; 53], [6; 0; 53], Accept); ([17; 0; 67], [17; 0; 67], Accept)]);
-   ("__map1", [([0; 0; 0; 2], [0; 0; 0; 2], Accept); ([0; 0; 0; 4], [0; 0; 0; 4], Accept); ([0; 0; 0; 1], [0; 0; 0; 1], Drop)]);
-   ("__map2", [([108; 111; 0; 0; 0; 0; 0; 0; 0; 0; 0; 0; 0; 0; 0; 0], [108; 111; 0; 0; 0; 0; 0; 0; 0; 0; 0; 0; 0; 0; 0; 0], Accept); ([112; 112; 112; 48; 0; 0; 0; 0; 0; 0; 0; 0; 0; 0; 0; 0], [112; 112; 112; 48; 0; 0; 0; 0; 0; 0; 0; 0; 0; 0; 0; 0], (Jump "inbound_world")); ([101; 116; 104; 49; 0; 0; 0; 0; 0; 0; 0; 0; 0; 0; 0; 0], [101; 116; 104; 49; 0; 0; 0; 0; 0; 0; 0; 0; 0; 0; 0; 0], (Jump "inbound_private"))]);
-   ("__map3", [([0; 0; 0; 2], [0; 0; 0; 2], Accept); ([0; 0; 0; 4], [0; 0; 0; 4], Accept); ([0; 0; 0; 1], [0; 0; 0; 1], Drop)])];
-   sd_maps := [] |}.
+Definition router_surface : sruleset :=
+  [TopNop;
+
+   (TopDefine "DEV_PRIVATE" (SVSym "eth1"));
+
+   (TopDefine "DEV_WORLD" (SVSym "ppp0"));
+
+   (TopDefine "NET_PRIVATE" (SVPrefix (sip4 192 168 0 0) 16));
+
+   (TopTable {| st_family := "ip"; st_name := "global";
+      st_items := [(TChain {| sc_name := "inbound_world";
+        sc_items := [(IRule [(CMatch {| sm_keys := [["ip"; "saddr"]]; sm_rhs := {| sr_op := SOpImplicit; sr_neg := false; sr_payload := (SSEvalue (sip4 81 209 165 42)) |} |});
+           (CMatch {| sm_keys := [["tcp"; "dport"]]; sm_rhs := {| sr_op := SOpImplicit; sr_neg := false; sr_payload := (SSEvalue (SVSym "ssh")) |} |});
+           (CVerdict SVaccept)])] |});
+      (TChain {| sc_name := "inbound_private";
+        sc_items := [(IRule [(CMatch {| sm_keys := [["icmp"; "type"]]; sm_rhs := {| sr_op := SOpImplicit; sr_neg := false; sr_payload := (SSEvalue (SVSym "echo-request")) |} |});
+           (CStmt (StLimit 5 "second" false 5 false));
+           (CVerdict SVaccept)]);
+         (IRule [(CVmap [["ip"; "protocol"]; ["th"; "dport"]] [((SVConcat [(SVSym "tcp"); (SVNum 22)]), SVaccept); ((SVConcat [(SVSym "udp"); (SVNum 53)]), SVaccept); ((SVConcat [(SVSym "tcp"); (SVNum 53)]), SVaccept); ((SVConcat [(SVSym "udp"); (SVNum 67)]), SVaccept)])])] |});
+      (TChain {| sc_name := "inbound";
+        sc_items := [(ITypeHook "filter" "input" false 0);
+         (IPolicy SVdrop);
+         (IRule [(CVmap [["ct"; "state"]] [((SVSym "established"), SVaccept); ((SVSym "related"), SVaccept); ((SVSym "invalid"), SVdrop)])]);
+         (IRule [(CVmap [["iifname"]] [((SVSym "lo"), SVaccept); ((SVVar "DEV_WORLD"), (SVjump "inbound_world")); ((SVVar "DEV_PRIVATE"), (SVjump "inbound_private"))])])] |});
+      (TChain {| sc_name := "forward";
+        sc_items := [(ITypeHook "filter" "forward" false 0);
+         (IPolicy SVdrop);
+         (IRule [(CVmap [["ct"; "state"]] [((SVSym "established"), SVaccept); ((SVSym "related"), SVaccept); ((SVSym "invalid"), SVdrop)])]);
+         (IRule [(CMatch {| sm_keys := [["iifname"]]; sm_rhs := {| sr_op := SOpImplicit; sr_neg := false; sr_payload := (SSEvalue (SVVar "DEV_PRIVATE")) |} |});
+           (CVerdict SVaccept)])] |});
+      (TChain {| sc_name := "postrouting";
+        sc_items := [(ITypeHook "nat" "postrouting" false 100);
+         (IPolicy SVaccept);
+         (IRule [(CMatch {| sm_keys := [["ip"; "saddr"]]; sm_rhs := {| sr_op := SOpImplicit; sr_neg := false; sr_payload := (SSEvalue (SVVar "NET_PRIVATE")) |} |});
+           (CMatch {| sm_keys := [["oifname"]]; sm_rhs := {| sr_op := SOpImplicit; sr_neg := false; sr_payload := (SSEvalue (SVVar "DEV_WORLD")) |} |});
+           (CStmt (StMasquerade []))])] |})] |})].
+
+Definition ifindex_pins (s : string) : option nat :=
+  if String.eqb s "lo" then Some 1%nat else None.
+
+Example router_lowers_ok : lower_ok ifindex_pins router_surface = true.
+Proof. vm_compute. reflexivity. Qed.
+
+Definition router_lowered : lowered_ruleset :=
+  Eval vm_compute in lower_or_empty ifindex_pins router_surface.
+
+Definition decls : set_decls := Eval vm_compute in lr_set_decls router_lowered.
 
 Definition base_env : env :=
   {| e_set := fun _ => []; e_vmap := fun _ => []; e_map := fun _ => [];
@@ -29,53 +70,23 @@ Definition gen_env : env := env_with_sets base_env decls.
 (* ===== table ip global ===== *)
 
 Definition global_inbound_world : chain :=
-  {| c_policy := Continue;
-   c_rules := [{| r_body := [(BMatch (elab_m (TMEq FIp4Saddr (ip4 81 209 165 42))));
-             (BDep (elab_m (TMEq FMetaL4proto (VInteger 1 6))));
-             (BMatch (elab_m (TMEq FThDport (VPort 22))))];
-     r_outcome := OVerdict Accept; r_after := [] |}] |}.
+  Eval vm_compute in lr_chain_of router_lowered "global" "inbound_world".
 
 Definition global_inbound_private : chain :=
-  {| c_policy := Continue;
-   c_rules := [{| r_body := [(BDep (elab_m (TMEq FMetaL4proto (VInteger 1 1))));
-             (BMatch (elab_m (TMEq FIcmpType (VInteger 1 8))));
-             (BMatch (MLimit {| ls_rate := 5; ls_unit := 0; ls_burst := 5; ls_bytes := false; ls_flags := 0 |}))];
-     r_outcome := OVerdict Accept; r_after := [] |};
-
-   {| r_body := [];
-     r_outcome := OVmap {| vm_fields := [FIp4Protocol; FThDport]; vm_keyf := None; vm_name := "__map0" |}; r_after := [] |}] |}.
+  Eval vm_compute in lr_chain_of router_lowered "global" "inbound_private".
 
 Definition global_inbound : chain :=
-  {| c_policy := Drop;
-   c_rules := [{| r_body := [];
-     r_outcome := OVmap {| vm_fields := []; vm_keyf := (Some (FCtState, [])); vm_name := "__map1" |}; r_after := [] |};
-
-   {| r_body := [];
-     r_outcome := OVmap {| vm_fields := []; vm_keyf := (Some (FMetaIifname, [])); vm_name := "__map2" |}; r_after := [] |}] |}.
+  Eval vm_compute in lr_chain_of router_lowered "global" "inbound".
 
 Definition global_forward : chain :=
-  {| c_policy := Drop;
-   c_rules := [{| r_body := [];
-     r_outcome := OVmap {| vm_fields := []; vm_keyf := (Some (FCtState, [])); vm_name := "__map3" |}; r_after := [] |};
-
-   {| r_body := [(BMatch (elab_m (TMEq FMetaIifname (ifname "eth1"))))];
-     r_outcome := OVerdict Accept; r_after := [] |}] |}.
+  Eval vm_compute in lr_chain_of router_lowered "global" "forward".
 
 Definition global_postrouting : chain :=
-  {| c_policy := Accept;
-   c_rules := [{| r_body := [(BMatch (elab_m (MPrefix FIp4Saddr CEq (ip4 192 168 0 0) 16)));
-             (BMatch (elab_m (TMEq FMetaOifname (ifname "ppp0"))))];
-     r_outcome := ONat {| nat_addr_imm := None; nat_field := None; nat_map := None; nat_src := None; nat_extra := NXnone; nat_kind := NKmasq; nat_family := NFip4; nat_flags := 0 |}; r_after := [] |}] |}.
+  Eval vm_compute in lr_chain_of router_lowered "global" "postrouting".
 
 Definition global_chains : list (string * chain) :=
-  [("inbound_world", global_inbound_world);
-   ("inbound_private", global_inbound_private);
-   ("inbound", global_inbound);
-   ("forward", global_forward);
-   ("postrouting", global_postrouting)].
+  Eval vm_compute in lr_chains_of router_lowered "global".
 
 Definition global_hooks : list hooked_chain :=
-  [{| hc_hook := Hinput; hc_prio := (0)%Z; hc_env := global_chains; hc_base := global_inbound |};
-   {| hc_hook := Hforward; hc_prio := (0)%Z; hc_env := global_chains; hc_base := global_forward |};
-   {| hc_hook := Hpostrouting; hc_prio := (100)%Z; hc_env := global_chains; hc_base := global_postrouting |}].
+  Eval vm_compute in lr_hooks_of router_lowered "global".
 
